utils/Zeta.Interleave.fsti
@@ -44,9 +44,19 @@ val per_thread_prefix (#a:_) (#n:_) (il: interleaving a n) (i:nat{i <= length il
 val i2s_map (#a:_) (#n:_) (il:interleaving a n) (i: SA.seq_index il)
   : (si:sseq_index (s_seq il){index il i = indexss (s_seq il) si /\ fst si = src il i})
 
+val i2s_map_monotonic (#a #n:_) (il: interleaving a n) (i j: SA.seq_index il)
+  : Lemma (requires (src il i = src il j))
+          (ensures ((i < j ==> snd (i2s_map il i) < snd (i2s_map il j)) /\
+                    (j < i ==> snd (i2s_map il j) < snd (i2s_map il i))))
+
 val s2i_map (#a:eqtype) (#n:_) (il:interleaving a n) (si: sseq_index (s_seq il)):
   (i: SA.seq_index il{index il i = indexss (s_seq il) si /\
-                  i2s_map il i = si})
+                      i2s_map il i = si /\ src il i = fst si})
+
+val s2i_map_monotonic (#a #n:_) (il: interleaving a n) (i j: sseq_index (s_seq il))
+  : Lemma (requires (fst i = fst j))
+          (ensures ((snd i < snd j ==> s2i_map il i < s2i_map il j) /\
+                    (snd j < snd i ==> s2i_map il j < s2i_map il i)))
 
 val lemma_i2s_s2i (#a:_) (#n:_) (il:interleaving a n) (i: SA.seq_index il):
   Lemma (ensures (s2i_map il (i2s_map il i) = i))
